sending side of HSL, now with sample HS code

src/tls/HSL.fst
@@ -11,7 +11,7 @@ open Hashing.CRF // now using incremental, collision-resistant, agile Hashing.
 module HH = FStar.HyperHeap
 module HS = FStar.HyperStack
 
-(* Handshake.Msg *) 
+(* A dummy Handshake.Msg *) 
 
 // simplified handshake messages; for this outline we show that the client 
 // agrees with the server on the two offers after checking the Finished message
@@ -36,6 +36,13 @@ let eoflight = function
 
 (* An outline of Handshake.Log *)
 
+(* TODO
+- add subregion discipline and the corresponding framing conditions
+- make prior ghost
+- add record-layer calls, keeping track of bytes buffers and their effective lengths
+- support abstract plaintexts and multiple epochs 
+*)
+
 let transcript_bytes ms = List.Tot.fold_left (fun a m -> a @| format m) empty_bytes ms
 // we will need to prove it is injective, we will rely in turn on concrete msg formats
 // should use a named lambda
@@ -48,9 +55,8 @@ assume val transcript_format_injective: ms0:list msg -> ms1:list msg ->
 assume val transcript_bytes_append: ms0: list msg -> ms1: list msg -> 
   Lemma (transcript_bytes (ms0 @ ms1) = transcript_bytes ms0 @| transcript_bytes ms1)
 
-
 // full specification of the hashed-prefix tags required for a given flight 
-// switching to a relational style to capture computational-hashed 
+// (in relational style to capture computational-hashed)
 val tags: a:alg -> prior: list msg -> ms: list msg -> hs: list (tag a) -> Tot Type0 (decreases ms)
 let rec tags a prior ms hs = 
   match ms with 
@@ -61,21 +67,8 @@ let rec tags a prior ms hs =
       | true, h::hs -> let t = transcript_bytes prior in (hashed a t /\ h == hash a t /\ tags a prior ms hs)
       | false, hs -> tags a prior ms hs
       | _ -> False 
-(* was:
-val tags: prior: list msg -> incoming: list msg -> Tot (list tag) (decreases incoming) 
-let rec tags prior incoming = 
-  match incoming with 
-  | [] -> [] 
-  | m :: ms -> 
-      let prior = List.Tot.append #msg prior [m] in
-      let rest = tags prior ms in 
-      if tagged m then 
-        hash (transcript_bytes prior) :: rest
-      else 
-        rest
-*) 
 
-val tags_nil_nil: a:alg -> prior: list msg -> Lemma (tags a prior [] [])
+private val tags_nil_nil: a:alg -> prior: list msg -> Lemma (tags a prior [] [])
 let tags_nil_nil a prior = ()
 
 //17-01-23 plausible ? 
@@ -88,80 +81,88 @@ let rec tags_append prior in0 in1 =
   | m :: ms -> ...
 *)      
 
-
 (* STATE *)
 
 //17-01-23 erasing the transcript involved many hide/reveal annotations and restrictions on embedding proofs in
 //17-01-23 stateful code. Besides, we need conditional ghosts... We may try again once the code is more stable.
-
-//17-02-06 TODO add some region discipline and the corresponding framing conditions
 noeq type state (a:alg) = | State:
   transcript: (*erased*) list msg -> // session transcript shared with the HS so far 
   input_msgs: list msg -> // partial incoming flight, hashed & parsed, with selected intermediate tags
   input_hashes: list (tag a) { tags a transcript input_msgs input_hashes } -> 
   hash: accv a { content hash = transcript_bytes (transcript @ input_msgs) } -> // current hash state
+  // output_bytes: buffer byte ->     // outgoing messages, already formatted and hashed.
+  // input_bytes: buffer byte ->       // received fragments; untrusted; not yet hashed or parsed
   state a
 type t (a:alg) = r:HS.ref (state a) // 17-01-19 HS naming!?
 
-val transcriptT: h:HS.mem -> #a:alg -> t a -> GTot (list msg) // the current transcript shared with the handshake
+//  specification-level transcript of all handshake messages logged so far
+val transcriptT: h:HS.mem -> #a:alg -> t a -> GTot (list msg) 
 let transcriptT h #a r = (HS.sel h r).transcript
 
-(*
-
-(*
-// type flight (prior:erased (list msg)) = ms:list msg & hs:list tag { hs = tags (reveal prior) ms }
-
-// internal state (although we may initially keep it transparent) 
-abstract type plainbytes i = bytes  // a shortcut: HSL merges handshake traffic at different indexes
-abstract type state = State
-  transcript: erased (list Msg.t) // session transcript shared with the HS so far 
-  output_bytes: buffer byte      // outgoing messages, already formatted and hashed.
-  input_bytes: buffer byte       // received fragments; untrusted; not yet hashed or parsed
-  input_msgs: flight  // partial incoming flight, hashed & parsed, with selected intermediate tags
-  hash: Hash.t { hash = HashA (transcript_bytes (List.Tot.append transcript input_msgs)) } // current hash state
-*)
-
-We will also need to keep track of lengths in the input/output buffers
-To separate between Reading and Writing modes, a precondition for sending a message should be that both input_bytes and input_msgs are empty. 
-(unclear who should check for emptyset, and how to react to extra bytes buffered past the input flight)
-*)
-
-(* commenting out the rest of the outline not used in the sample code for now: 
-
-type t  // a stateful instance of HS log, including I/O buffers
-
-val writing: mem -> t -> GTot bool // can we currently send a HS message? 
-
-// Flights are delimited by changes either of epoch or direction.
-*)
+// specification-level guard for sending: we have not started receiving the next flight
+val writing: h:HS.mem -> #a:alg -> t a -> GTot bool 
+let writing h #a r = List.Tot.isEmpty (HS.sel h r).input_msgs
 
 val create: a:alg -> ST (t a) 
   (requires (fun h0 -> True))
   (ensures (fun h0 r h1 -> // "allocated in r" /\ writing h1 r /\ 
+    writing h1 r /\  
     transcriptT h1 r == []))
 let create a = 
   let v = Hashing.start a in 
   ST.ralloc HH.root (State [] [] [] v)
   
-// We send one message at a time (or in two steps for CH); for simplicity we distinguish between tagged and untagged.
+// We send one message at a time (or in two steps for CH); 
+// for call-site simplicity we distinguish between tagged and untagged messages
+// We require ms_0 be empty; otherwise the hash computation is messed up
 
 val send: #a:alg -> r:t a -> m:msg {~(tagged m)} -> ST unit 
   (requires (fun h0 -> 
-    True //writing h0 t
+    writing h0 r
   )) 
   (ensures (fun h0 _ h1 -> 
+    writing h1 r /\
     transcriptT h1 r == transcriptT h0 r @ [m] 
   ))
-(* // we need writing to ensure ms_0 is empty; otherwise the hash computation is messed up
 let send #a r m = 
-  let State prior_0 ms_0 hs_0 v_0 = !r in
+  let State prior_0 [] hs_0 v_0 = !r in // using pattern matching to assert ms = [] 
   let bs = format m in
   let v_1 = extend v_0 bs in 
   let prior_1 = prior_0 @ [m] in 
   let hs_1 = hs_0 @ [] in
-  r := State prior ms_1 hs_1 v_1
-*)
-  
+  List.Tot.append_assoc prior_0 [m] [];
+  List.Tot.append_assoc prior_0 [] [m];
+  transcript_bytes_append (prior_0 @ []) [m];
+  assert_norm(Seq.equal (transcript_bytes [m]) bs);
+  ST.recall r;
+  r := State prior_1 [] hs_1 v_1
+
+val send_tag: #a:alg -> r:t a -> m:msg {tagged m} -> ST (tag a)
+  (requires (fun h0 -> 
+    writing h0 r
+  )) 
+  (ensures (fun h0 h h1 -> 
+    let t_0 = transcriptT h0 r in 
+    let t_1 = transcriptT h1 r in 
+    let bs = transcript_bytes t_1 in
+    writing h1 r /\
+    t_1 == t_0 @ [m] /\
+    hashed a bs /\ h == hash a bs
+  ))
+let send_tag #a r m = 
+  let State prior_0 [] hs_0 v_0 = !r in // using pattern matching to assert ms = [] 
+  let bs = format m in
+  let v_1 = extend v_0 bs in 
+  let h = finalize v_1 in 
+  let prior_1 = prior_0 @ [m] in 
+  let hs_1 = hs_0 in
+  List.Tot.append_assoc prior_0 [m] [];
+  List.Tot.append_assoc prior_0 [] [m];
+  transcript_bytes_append (prior_0 @ []) [m];
+  assert_norm(Seq.equal (transcript_bytes [m]) bs);
+  ST.recall r;
+  r := State prior_1 [] hs_1 v_1;
+  h
 
 (*
 // For the record layer (no effect on the abstract HS state)
@@ -169,17 +170,19 @@ val next_fragment: t -> i:id -> ST (option fragment)
   (ensures (fun h0 r h1 -> transcript h0 t = transcript h1 t)) 
 *)
 
-// We receive messages in whole flights 
+// We receive messages in whole flights; 
+// note that, untill a full flight is received, we lose "writing h1 r"
 val receive: #a:alg -> r:t a -> bytes -> ST (option (list msg * list (tag a)))
   (requires (fun h0 -> True))
   (ensures (fun h0 o h1 -> 
     let t0 = transcriptT h0 r in
     let t1 = transcriptT h1 r in
     match o with 
-    | Some (ms, hs) -> t1 == t0 @ ms /\ tags a t0 ms hs
+    | Some (ms, hs) -> t1 == t0 @ ms /\ tags a t0 ms hs /\ writing h1 r
     | None -> t1 == t0
   ))
 
+#reset-options "--z3rlimit 40" 
 let receive #a r bs = 
   match parse_msg bs with // assuming bs is a potential whole message
   | None -> None
@@ -188,7 +191,7 @@ let receive #a r bs =
       let ms_1 = ms_0 @ [m]  in
       let content_0 = transcript_bytes (prior @ ms_0) in 
       let content_1 = transcript_bytes (prior @ ms_1) in 
-      FStar.List.Tot.Properties.append_assoc prior ms_0 [m];
+      List.Tot.append_assoc prior ms_0 [m];
 
       transcript_bytes_append (prior@ms_0) [m];
       assert_norm(Seq.equal (transcript_bytes [m]) (format m));
@@ -196,7 +199,7 @@ let receive #a r bs =
       // assert(content v_1 == content_1);
 
       let hs' = if tagged m then [finalize v_1] else [] in
-      assert(tags a (prior@ms_0) [m] hs');
+      assert(tags a (prior@ms_0) [m] hs'); //17-02-06 this assert is brittle, why?
       assert(tags a prior ms_0 hs_0); 
       tags_append a prior ms_0 [m] hs_0 hs';
       let hs_1 = hs_0 @ hs' in
@@ -206,7 +209,7 @@ let receive #a r bs =
       if eoflight m then  
         let prior_1 = prior @ ms_1 in 
         ( tags_nil_nil a prior_1; 
-          FStar.List.Tot.Properties.append_l_nil prior_1; // seems necessary...
+          List.Tot.append_l_nil prior_1; // seems necessary...
           // assert(prior_1 @ [] == prior @ ms_1);
           // assert(content v_1 == transcript_bytes (prior_1 @ []));
           r := State prior_1 [] [] v_1; 
@@ -214,23 +217,22 @@ let receive #a r bs =
       else (
         r := State prior ms_1 hs_1 v_1; 
         None ))
+#reset-options ""
 
+(* An outline of Handshake, to check usability *) 
 
-(*
-design: ghost log vs forall log?
-design: how to return flights with intermediate tags?
-TODO: support multiple epochs? 
-*)
-
-////// An outline of Handshake
-
-assume val nego: offer -> GTot offer // the server's choice of parameters
+assume val nego: offer -> Tot offer // the server's choice of parameters
 assume val mac_verify: a:alg -> h:tag a -> t:tag SHA256-> 
 // in existential style, did not manage to trigger on offer.
 //  Tot (b:bool { b ==> (exists offer.  h = hash(transcript_bytes [ClientHello offer; ServerHello (nego offer)])) })
   Tot (b:bool { b ==> (forall c s.  
     let tr = transcript_bytes [ClientHello c; ServerHello s] in 
     (hashed a tr /\ h = hash a tr ==> s == nego c)) })
+
+assume val mac_compute: a:alg -> h:tag a -> Tot (t:tag SHA256
+  { forall c s.  
+    let tr = transcript_bytes [ClientHello c; ServerHello s] in 
+    (hashed a tr /\ h = hash a tr ==> s == nego c) })
 
 (*
 let inj_format c0 s0 c1 s1 : Lemma ( 
@@ -244,8 +246,31 @@ noeq type result 'a =
   | Error of string 
   | Retry
 
+val server_process: #a:alg -> log: t a -> bytes -> ST (result (offer * offer * tag SHA256)) 
+  (requires (fun h0 -> 
+    transcriptT h0 log == []))
+  (ensures (fun h0 r h1 -> 
+    match r with 
+    | Result (c,s,t) -> 
+        //(exists (c:offer) (t:tag SHA256). s == nego c /\ transcriptT h1 log == [ClientHello c; ServerHello s; Finished t])
+        s == nego c /\ transcriptT h1 log == [ClientHello c; ServerHello s; Finished t]
+    | Retry -> transcriptT h1 log == transcriptT h0 log 
+    | Error _ -> True))
+#reset-options "--z3rlimit 100"
+let server_process #a log (raw:bytes) = 
+  match receive log raw with 
+  | None -> Retry
+  | Some ([ClientHello c], []) -> (
+      let s = nego c in
+      let h = send_tag log (ServerHello s) in
+      let t = mac_compute a h in
+      //assert_norm([]@[ClientHello c]@[ServerHello s]@[Finished t] == [ClientHello c; ServerHello s; Finished t]);
+      send log (Finished t);
+      Result (c,s,t))
+  | _ -> Error "bad Flight"
+
 // the HS handler for receiving the server flight after sending a client offer
-val process: a:alg -> log:t a -> bytes -> c:offer -> ST (result offer)
+val client_process: #a:alg -> log:t a -> bytes -> c:offer -> ST (result offer)
   (requires (fun h0 -> 
     transcriptT h0 log == [ClientHello c]))
   (ensures (fun h0 r h1 -> 
@@ -253,7 +278,7 @@ val process: a:alg -> log:t a -> bytes -> c:offer -> ST (result offer)
     | Result s -> ( s == nego c /\ (exists (t:tag SHA256). transcriptT h1 log == [ClientHello c; ServerHello s; Finished t]))
     | Retry -> transcriptT h1 log == transcriptT h0 log 
     | Error _ -> True))
-let process a log (raw:bytes) c = 
+let client_process #a log (raw:bytes) c = 
   match receive log raw with 
   | None -> Retry
   | Some ([ServerHello s; Finished t], [hash_ch_sh]) -> 
